theories/LambdaWt/DepUtil.v
@@ -1,0 +1,272 @@
+Require Import ExtLib.Data.Member.
+Require Import ExtLib.Data.HList.
+Require Import ExtLib.Tactics.
+
+Set Implicit Arguments.
+Set Strict Implicit.
+
+Section hlist_Forall.
+  Context {T : Type} {F G : T -> Type}.
+  Variable P : forall t, F t -> Prop.
+  Inductive hlist_Forall : forall ts, hlist F ts -> Prop :=
+  | hlist_Forall_nil : @hlist_Forall nil Hnil
+  | hlist_Forall_cons : forall t ts x xs,
+      @P t x ->
+      @hlist_Forall ts xs ->
+      @hlist_Forall (t :: ts) (Hcons x xs).
+
+  Variable R : forall t, F t -> G t -> Prop.
+  Inductive hlist_Forall2 : forall ts, hlist F ts -> hlist G ts -> Prop :=
+  | hlist_Forall2_nil : @hlist_Forall2 nil Hnil Hnil
+  | hlist_Forall2_cons : forall t ts x xs y ys,
+      @R t x y ->
+      @hlist_Forall2 ts xs ys ->
+      @hlist_Forall2 (t :: ts) (Hcons x xs) (Hcons y ys).
+End hlist_Forall.
+Arguments hlist_Forall_nil {_ _ _}.
+Arguments hlist_Forall_cons {_ _ _ _ _ _ _} _ _.
+
+Section Forall2.
+  Context {T U : Type}.
+  Variable P : T -> U -> Prop.
+  Inductive Forall2 : list T -> list U -> Prop :=
+  | Forall2nil : Forall2 nil nil
+  | Forall2cons : forall x xs y ys, P x y -> Forall2 xs ys ->
+                                    Forall2 (x :: xs) (y :: ys).
+End Forall2.
+
+Section hlist_Forall2.
+  Context {T : Type} {F : T -> Type} {G : forall x, F x -> F x -> Prop}
+          (P : forall x (a b : F x), G x a b -> Prop).
+
+  Variable R : forall t (a b : F t), G a b -> Prop.
+  Inductive hlist_Forall2_dep
+    : forall ts (a b : hlist F ts), hlist_Forall2 G a b -> Prop :=
+  | hlist_Forall2_dep_nil :
+      @hlist_Forall2_dep nil Hnil Hnil (@hlist_Forall2_nil _ _ _ _)
+  | hlist_Forall2_dep_cons : forall t ts x xs y ys pf pfs,
+      P pf ->
+      @hlist_Forall2_dep ts xs ys pfs ->
+      @hlist_Forall2_dep (t :: ts) (Hcons x xs) (Hcons y ys)
+                         (@hlist_Forall2_cons T F F G t ts _ _ _ _ pf pfs).
+
+End hlist_Forall2.
+
+(** * Auxiliary Functions **)
+
+Section member_eq_dec.
+  Context {T : Type}.
+  Context {T_dec : forall a b : T, {a = b} + {a <> b}}.
+  Fixpoint member_eq_dec ts (t : T) (a : member t ts)
+    : forall b,  {a = b} + {a <> b}.
+    refine
+      match a in member _ ts
+            return forall b : member t ts, {a = b} + {a <> b}
+      with
+      | MZ _ _ => fun b =>
+                    match b as b in member _ (t' :: l)
+                          return forall pf : t' = t,
+                        {MZ t l = match pf with
+                                  | eq_refl => b
+                                  end} +
+                        {MZ t l <> match pf with
+                                   | eq_refl => b
+                                   end}
+                    with
+                    | MZ _ ls => fun pf => left _
+                    | MN _ _ => fun pf => right _
+                    end eq_refl
+      | MN _ m => fun b =>
+                    match b as b in member _ (t' :: l)
+                          return forall m, (forall x, {m = x} + {m <> x}) ->
+                                           {MN _ m = b} + {MN _ m <> b}
+                    with
+                    | MZ _ _ => fun _ _ => right _
+                    | MN _ m => fun _ rec => match rec m with
+                                             | left pf => left _
+                                             | right pf => right _
+                                             end
+                    end m (fun x => member_eq_dec _ _ m x)
+      end.
+    destruct (eq_sym (UIP_refl pf)). reflexivity.
+    clear - pf. subst. intro. inversion H.
+    clear. intro. inversion H.
+    f_equal. assumption.
+    clear - pf T_dec. intro. apply pf. inversion H.
+    eapply Eqdep_dec.inj_pair2_eq_dec in H1. assumption.
+    eapply List.list_eq_dec. eassumption.
+    Unshelve. eapply T_dec.
+  Defined.
+
+  Require Import Coq.Lists.List.
+
+  Section with_t.
+    Context {t : T}.
+    Fixpoint member_weaken {ls} ls'
+      : member t ls -> member t (ls' ++ ls) :=
+      match ls' as ls'
+            return member t ls -> member t (ls' ++ ls)
+      with
+      | nil => fun x => x
+      | l :: ls' => fun x => MN _ (member_weaken ls' x)
+      end.
+
+    Fixpoint member_lift ls ls' ls''
+      : member t (ls'' ++ ls) -> member t (ls'' ++ ls' ++ ls) :=
+      match ls'' as ls''
+            return member t (ls'' ++ ls) -> member t (ls'' ++ ls' ++ ls)
+      with
+      | nil => member_weaken ls'
+      | l :: ls'' => fun m =>
+                       match m in member _ (x :: xs)
+                             return forall xs', (member t xs -> member t xs') ->
+                                                member t (x :: xs')
+                       with
+                       | MZ _ _ => fun _ _ => MZ _ _
+                       | MN _ m => fun _ rec => MN _ (rec m)
+                       end _ (member_lift  ls ls' ls'')
+      end.
+  End with_t.
+End member_eq_dec.
+
+Section hlist_eq_dec.
+  Context {T : Type} {F : T -> Type}.
+  Variable F_dec : forall t (a b : F t), {a = b} + {a <> b}.
+  Fixpoint hlist_eq_dec {ls} (a : hlist F ls)
+    : forall b : hlist F ls, {a = b} + {a <> b}.
+    refine
+      match a as a in hlist _ ls
+            return forall b : hlist F ls, {a = b} + {a <> b}
+      with
+      | Hnil => fun x => left _
+      | Hcons x xs => fun b =>
+                        match F_dec x (hlist_hd b)
+                              , hlist_eq_dec _ xs (hlist_tl b)
+                        with
+                        | left pf , left pf' => left _
+                        | _ , _ => right _
+                        end
+      end.
+    { symmetry. apply (hlist_eta x). }
+    { rewrite hlist_eta. congruence. }
+    { clear - n. intro; subst. simpl in *. auto. }
+    { clear - n. intro; subst. simpl in *. auto. }
+  Defined.
+End hlist_eq_dec.
+
+(** TODO(gmalecha): Move to ExtLib **)
+Definition pair_eq_dec {T U} (T_dec : forall a b : T, {a = b} + {a <> b})
+           (U_dec : forall a b : U, {a = b} + {a <> b})
+  : forall a b : T * U, {a = b} + {a <> b}.
+  refine
+    (fun a b =>
+       match a as a , b as b with
+       | (l,r) , (l',r') => match T_dec l l' , U_dec r r' with
+                            | left pf , left pf' => left _
+                            | _ , _ => right _
+                            end
+       end); subst; auto. congruence. congruence.
+Defined.
+
+Section hlist_map_rules.
+  Variable A : Type.
+  Variables F G G' : A -> Type.
+  Variable ff : forall x, F x -> G x.
+  Variable gg : forall x, G x -> G' x.
+
+  Theorem hlist_map_hlist_map : forall ls (hl : hlist F ls),
+      hlist_map gg (hlist_map ff hl) = hlist_map (fun _ x => gg (ff x)) hl.
+  Proof.
+    induction hl; simpl; f_equal. assumption.
+  Defined.
+
+  Theorem hlist_get_hlist_map : forall ls t (hl : hlist F ls) (m : member t ls),
+      hlist_get m (hlist_map ff hl) = ff (hlist_get m hl).
+  Proof.
+    induction m; simpl.
+    { rewrite (hlist_eta hl). reflexivity. }
+    { rewrite (hlist_eta hl). simpl. auto. }
+  Defined.
+
+  Lemma hlist_map_ext : forall (ff gg : forall x, F x -> G x),
+      (forall x t, ff x t = gg x t) ->
+      forall ls (hl : hlist F ls),
+        hlist_map ff hl = hlist_map gg hl.
+  Proof.
+    induction hl; simpl; auto.
+    intros. f_equal; auto.
+  Defined.
+
+End hlist_map_rules.
+
+Lemma hlist_get_member_weaken:
+  forall {T : Type} (F : T -> Type) (tvs tvs' : list T) (t0 : T) (m : member t0 tvs) (vs : hlist F tvs) (vs' : hlist F tvs'),
+    hlist_get (member_weaken tvs' m) (hlist_app vs' vs) = hlist_get m vs.
+Proof.
+  clear.
+  induction tvs'; simpl; intros.
+  { rewrite (hlist_eta vs'). reflexivity. }
+  { rewrite (hlist_eta vs'). simpl. eauto. }
+Qed.
+
+Lemma hlist_get_member_lift
+: forall T (F : T -> Type) (tvs tvs' tvs0 : list T) (t0 : T) (m : member t0 (tvs0 ++ tvs)) (vs : hlist F tvs)
+         (vs' : hlist F tvs') (vs'' : hlist F tvs0),
+    hlist_get (member_lift tvs tvs' tvs0 m) (hlist_app vs'' (hlist_app vs' vs))
+    = hlist_get m (hlist_app vs'' vs).
+Proof.
+  clear.
+  induction vs''.
+  { simpl in *.
+    eapply hlist_get_member_weaken. }
+  { destruct (member_case m).
+    { destruct H. subst. reflexivity. }
+    { destruct H. subst. eapply IHvs''. } }
+Qed.
+
+(*
+Lemma hlist_get_member_lift'
+  : forall tus tvsX tvs tvs' tvs''
+           (xs : hlist (wtexpr tus tvsX) tvs)
+           (xs' : hlist (wtexpr tus tvsX) tvs')
+           (xs'' : hlist (wtexpr tus tvsX) tvs'')
+           t Z
+           (pf : Z = (List.app tvs'' tvs))
+           (m : member t Z),
+    hlist_get (member_lift tvs tvs' tvs'' match pf with
+                                          | eq_refl => m
+                                          end) (hlist_app xs'' (hlist_app xs' xs)) =
+    hlist_get match pf with
+              | eq_refl => m
+              end (hlist_app xs'' xs).
+Proof using.
+  clear.
+  induction tvs''; simpl.
+  { intros; subst. rewrite (hlist_eta xs''). simpl.
+    clear.
+    induction xs'.
+    { reflexivity. }
+    { simpl. eauto. } }
+  { clear - IHtvs''.
+    intros; subst.
+    destruct (member_case m).
+    { destruct H. subst. simpl. rewrite (hlist_eta xs'').
+      reflexivity. }
+    { destruct H. subst. simpl. rewrite (hlist_eta xs''). simpl.
+      specialize (IHtvs'' xs xs' (hlist_tl xs'') t _ eq_refl).
+      simpl in *. eauto. } }
+Qed.
+
+Lemma hlist_get_member_lift
+  : forall tus tvsX tvs tvs' tvs''
+           (xs : hlist (wtexpr tus tvsX) tvs)
+           (xs' : hlist (wtexpr tus tvsX) tvs')
+           (xs'' : hlist (wtexpr tus tvsX) tvs'')
+           t
+           (m : member t (List.app tvs'' tvs)),
+    hlist_get (member_lift tvs tvs' tvs'' m) (hlist_app xs'' (hlist_app xs' xs)) =
+    hlist_get m (hlist_app xs'' xs).
+Proof using.
+  intros. eapply hlist_get_member_lift' with (pf:=eq_refl).
+Qed.
+*)
