theories/LambdaWt/WtMigrator.v
@@ -1,0 +1,221 @@
+Require Import Coq.Lists.List.
+Require Import ExtLib.Structures.Applicative.
+Require Import ExtLib.Data.Member.
+Require Import ExtLib.Data.HList.
+Require Import ExtLib.Tactics.
+Require Import MirrorCore.LambdaWt.WtType.
+Require Import MirrorCore.LambdaWt.WtExpr.
+
+Set Implicit Arguments.
+Set Strict Implicit.
+
+(* This is the universe of the reified language *)
+Universe Urefl.
+
+Section simple_dep_types.
+  Variable Tsymbol : Type.
+  Variable TsymbolD : Tsymbol -> Type@{Urefl}.
+
+  Variable Esymbol : type Tsymbol -> Type.
+  Variable EsymbolD : forall t, Esymbol t -> typeD TsymbolD t.
+
+  (** Instantiation **)
+  Definition migrator (tus tus' : list (Tuvar Tsymbol)) : Type :=
+    hlist (fun tst => wtexpr Esymbol tus' (fst tst) (snd tst)) tus.
+
+  Definition migrator_tl
+  : forall {a b c} (mig : migrator (b :: c) a),
+      migrator c a := fun _ => @hlist_tl _ _.
+
+  Definition migrate_env {tus tus'}
+             (mig : migrator tus' tus) (e : Uenv TsymbolD tus)
+  : Uenv TsymbolD tus' := Eval cbv beta in
+    hlist_map (fun _ val => wtexprD EsymbolD val e) mig.
+
+  Section migrate_expr.
+    Context {tus tus'} (mig : migrator tus tus').
+
+    Fixpoint migrate_expr {tvs t}
+             (e : wtexpr Esymbol tus tvs t)
+    : wtexpr Esymbol tus' tvs t :=
+      match e in wtexpr _ _ _ t
+            return wtexpr _ tus' tvs t
+      with
+      | wtVar v => wtVar v
+      | wtInj v => wtInj v
+      | wtApp f x => wtApp (migrate_expr f) (migrate_expr x)
+      | wtAbs e => wtAbs (migrate_expr e)
+      | wtUVar u vs => subst (hlist_map (@migrate_expr tvs) vs) (hlist_get u mig)
+      end.
+  End migrate_expr.
+
+  Fixpoint migrator_compose {tus tus' tus''}
+           (mig : migrator tus tus')
+           (mig' : migrator tus' tus'')
+  : migrator tus tus'' :=
+    match mig in hlist _ tus
+          return migrator tus tus''
+    with
+    | Hnil => Hnil
+    | @Hcons _ _ l ls e mig'0 => Hcons (migrate_expr mig' e) (migrator_compose mig'0 mig')
+    end.
+
+  Theorem migrate_env_migrate_expr
+  : forall tus tus' tvs t (mig : migrator tus tus')
+           (e : wtexpr Esymbol tus tvs t),
+      forall us vs,
+        wtexprD EsymbolD (migrate_expr mig e) us vs =
+        wtexprD EsymbolD e (migrate_env mig us) vs.
+  Proof.
+    induction e.
+    { simpl. unfold Var_exprT. reflexivity. }
+    { simpl. unfold Pure_exprT. reflexivity. }
+    { simpl. unfold Ap_exprT. intros.
+      rewrite IHe1. rewrite IHe2. reflexivity. }
+    { simpl. unfold Abs_exprT. intros.
+      eapply FunctionalExtensionality.functional_extensionality.
+      intros. eapply IHe. }
+    { simpl. intros. unfold UVar_exprT.
+      unfold migrate_env at 1.
+      rewrite hlist_get_hlist_map.
+      generalize (hlist_get u mig); simpl.
+      rewrite hlist_map_hlist_map.
+      intros. rewrite wtexprD_subst.
+      rewrite hlist_map_hlist_map.
+      f_equal.
+      clear - H.
+      induction H; simpl.
+      - reflexivity.
+      - f_equal; eauto. }
+  Qed.
+
+  Section mid.
+    Variable T : Tuvar Tsymbol -> Type.
+
+    Local Fixpoint migrator_id' (tus : list (Tuvar Tsymbol)) {struct tus}
+    : (forall ts t, member (ts,t) tus -> T (ts,t)) ->
+      hlist T tus :=
+      match tus as tus
+            return (forall ts t, member (ts,t) tus -> T (ts,t)) ->
+                   hlist T tus
+      with
+      | nil => fun _ => Hnil
+      | (ts,t) :: tus => fun mk =>
+                           Hcons (@mk _ _ (@MZ _ _ _))
+                                 (migrator_id' (fun ts t z => @mk ts t (MN _ z)))
+      end.
+  End mid.
+
+  Local Fixpoint vars_id {tus} tvs
+  : hlist (wtexpr Esymbol tus tvs) tvs :=
+    match tvs as tvs
+          return hlist (wtexpr Esymbol tus tvs) tvs
+    with
+    | nil => Hnil
+    | t :: ts =>
+      Hcons (wtVar (MZ t ts))
+            (hlist_map
+               (fun t' : type Tsymbol => wtexpr_lift (t :: nil) nil)
+               (vars_id ts))
+    end.
+
+  Definition migrator_id tus : migrator tus tus :=
+    @migrator_id' _ tus (fun ts t x => wtUVar x (vars_id ts)).
+  Arguments migrator_id {tus} : rename.
+
+  Lemma hlist_get_migrator_id'
+  : forall T ts t tus mk (m : member (ts,t) tus),
+      hlist_get m (@migrator_id' T tus mk) = mk _ _ m.
+  Proof.
+    induction m; simpl; auto.
+    destruct l. simpl. rewrite IHm. reflexivity.
+  Qed.
+
+  Lemma hlist_get_migrator_id
+  : forall ts t tus (m : member (ts,t) tus),
+      hlist_get m (migrator_id (tus:=tus)) = wtUVar m (vars_id _).
+  Proof.
+    intros. unfold migrator_id.
+    rewrite hlist_get_migrator_id'. reflexivity.
+  Qed.
+
+  Theorem migrate_expr_migrator_id
+  : forall tus tvs t (e : wtexpr _ tus tvs t),
+      migrate_expr migrator_id e = e.
+  Proof.
+    induction e; simpl; intros; auto.
+    { rewrite IHe1. rewrite IHe2. reflexivity. }
+    { rewrite IHe. reflexivity. }
+    { rewrite hlist_get_migrator_id. simpl.
+      f_equal.
+      clear - H.
+      induction H; simpl; auto.
+      f_equal; eauto.
+      etransitivity; [ | eassumption ].
+      rewrite hlist_map_hlist_map.
+      eapply hlist_map_ext.
+      intros.
+      rewrite <- IHhlist_Forall.
+      rewrite hlist_map_hlist_map.
+      eapply (fun Z => @subst_wtexpr_lift _ _ tus nil _ _ t0 (t :: nil) _
+                                          Hnil (Hcons Z Hnil)). }
+  Qed.
+
+  Lemma hlist_map_vars_id_id
+  : forall (p : _) (x : Venv TsymbolD p)
+           (l : list (Tuvar Tsymbol))
+           (h : hlist
+                  (fun tst : Tuvar Tsymbol =>
+                     hlist (typeD TsymbolD) (fst tst) ->
+                     typeD TsymbolD (snd tst)) l),
+      hlist_map
+        (fun (x0 : type Tsymbol) (x1 : wtexpr Esymbol l p x0) =>
+           wtexprD EsymbolD x1 h x) (vars_id p) = x.
+  Proof.
+    induction x; simpl; auto.
+    { intros. f_equal. rewrite hlist_map_hlist_map.
+      etransitivity; [ | eapply IHx ].
+      eapply hlist_map_ext.
+      intros.
+      erewrite wtexprD_wtexpr_lift
+      with (vs'':=Hnil) (vs':=Hcons f Hnil) (vs:=x).
+      reflexivity. }
+  Qed.
+
+  (** TODO(gmalecha): Move to ExtLib.Data.HList *)
+  Lemma hlist_ext : forall T (F : T -> Type) (ls : list T)
+                           (a b : hlist F ls),
+      (forall t (m : member t ls), hlist_get m a = hlist_get m b) ->
+      a = b.
+  Proof using.
+    clear.
+    induction a; intros.
+    { rewrite (hlist_eta b). reflexivity. }
+    { rewrite (hlist_eta b).
+      f_equal.
+      { eapply (H _ (MZ _ _)). }
+      { eapply IHa.
+        intros. eapply (H _ (MN _ _)). } }
+  Defined.
+
+  Lemma migrate_env_migrator_id
+  : forall tus (e : Uenv TsymbolD tus),
+      migrate_env migrator_id e = e.
+  Proof using.
+    intros.
+    eapply hlist_ext; intros.
+    unfold migrate_env.
+    rewrite hlist_get_hlist_map.
+    destruct t.
+    rewrite hlist_get_migrator_id with (m:=m).
+    simpl. unfold UVar_exprT.
+    eapply FunctionalExtensionality.functional_extensionality; intros.
+    rewrite hlist_map_hlist_map.
+    rewrite hlist_map_vars_id_id.
+    reflexivity.
+  Qed.
+
+End simple_dep_types.
+
+Arguments migrator {_} _ _ _.
+Arguments migrator_id {_ _ tus}.
