theories/LambdaWt/WtType.v
@@ -1,0 +1,60 @@
+Require Import ExtLib.Structures.Applicative.
+Require Import ExtLib.Data.Member.
+Require Import ExtLib.Data.HList.
+Require Import ExtLib.Tactics.
+
+Set Implicit Arguments.
+Set Strict Implicit.
+
+(* This is the universe of the reified language *)
+Universe Urefl.
+
+Section simple_dep_types.
+  Variable Tsymbol : Type.
+  Variable TsymbolD : Tsymbol -> Type@{Urefl}.
+
+  Inductive type : Type :=
+  | TArr : type -> type -> type
+  | TInj : Tsymbol -> type.
+
+  Fixpoint typeD (t : type) : Type@{Urefl} :=
+    match t with
+    | TArr a b => typeD a -> typeD b
+    | TInj s => TsymbolD s
+    end.
+
+  Variable Tsymbol_eq_dec : forall a b : Tsymbol, {a = b} + {a <> b}.
+
+  (** TODO: If we move to a weaker notion of types, e.g. with reduction,
+   ** we're going to need a weaker equivalence relation
+   **)
+  Fixpoint type_eq_dec (t t' : type) : {t = t'} + {t <> t'}.
+  refine
+    match t as t , t' as t' return {t = t'} + {t <> t'} with
+    | TInj a , TInj b => match Tsymbol_eq_dec a b with
+                         | left pf => left (f_equal _ pf)
+                         | right pf => right _
+                         end
+    | TArr d c , TArr d' c' => match type_eq_dec d d'
+                                   , type_eq_dec c c'
+                               with
+                               | left pf , left pf' => left _
+                               | _ , _ => right _
+                               end
+    | _ , _ => right _
+    end; try congruence.
+  Defined.
+
+  Definition codom (t : type) : type :=
+    match t with
+    | TArr _ c => c
+    | _ => t
+    end.
+
+  Definition dom (t : type) : type :=
+    match t with
+    | TArr d _ => d
+    | _ => t
+    end.
+
+End simple_dep_types.
